task: add small step semantics and prove correct

ArithJetbrains/Basic.lean
@@ -12,12 +12,14 @@ inductive Result (α : Type) where
   | ok : α → Result α
   | divByZero : Result α
 
+@[simp]
 instance : Monad Result where
   pure := Result.ok
   bind
     | Result.ok n, f => f n
     | Result.divByZero, _ => Result.divByZero
 
+@[simp]
 def eval : Term → Result Nat
   | .const n => pure n
   | .op op t1 t2 =>
@@ -31,3 +33,44 @@ def eval : Term → Result Nat
 
 #eval eval (Term.op .add (Term.const 5) (Term.op .mul (Term.const 2) (Term.const 3))) -- 11
 #eval eval (Term.op .div (Term.const 10) (Term.op .sub (Term.const 5) (Term.const 5))) -- divByZero
+
+
+inductive Step : Term -> Term -> Prop where
+  | opCtx1 : ∀ op t1 t1' t2,
+      Step t1 t1' →
+      Step (Term.op op t1 t2) (Term.op op t1' t2)
+  | opCtx2 : ∀ op n1 t2 t2',
+      Step t2 t2' →
+      Step (Term.op op (.const n1) t2) (Term.op op (.const n1) t2')
+  | addConst : ∀ n1 n2,
+      Step (Term.op .add (.const n1) (.const n2)) (.const (n1 + n2))
+  | subConst : ∀ n1 n2,
+      Step (Term.op .sub (.const n1) (.const n2)) (.const (n1 - n2))
+  | mulConst : ∀ n1 n2,
+      Step (Term.op .mul (.const n1) (.const n2)) (.const (n1 * n2))
+  | divConst : ∀ n1 n2,
+      n2 ≠ 0 →
+      Step (Term.op .div (.const n1) (.const n2)) (.const (n1 / n2))
+
+-- reflexive transitive closure of Step
+inductive StepStar : Term -> Term -> Prop where
+  | refl : ∀ t, StepStar t t
+  | trans : ∀ t1 t2 t3, Step t1 t2 → StepStar t2 t3 → StepStar t1 t3
+
+-- reducing a term does not affect its evaluation
+theorem step_eval : ∀ t t',
+    Step t t' →
+    eval t = eval t' := by
+    intro t t' h
+    induction h <;> simp [*]
+
+-- correctness of the small-step semantics
+theorem step_correct : ∀ t t' n,
+    StepStar t t' →
+    t' = Term.const n →
+    eval t = Result.ok n := by
+  intro t t' n h ht'
+  induction h with
+  | refl => intros; subst ht'; rfl
+  | trans t1 t2 t3 hstep hstar ih =>
+      rw [step_eval _ _ hstep, ih ht']
